Fix an issue with the names of the loop decreases clauses

tests/fstar/misc/Loops.Clauses.fst
@@ -6,103 +6,103 @@ open Loops.Types
 #set-options "--z3rlimit 50 --fuel 1 --ifuel 1"
 
 (** [loops::sum]: decreases clause *)
-unfold let sum_decreases (max : u32) (i : u32) (s : u32) : nat =
+unfold let sum_loop_decreases (max : u32) (i : u32) (s : u32) : nat =
   if i <= max then max - i else 0
 
 (** [loops::sum_with_mut_borrows]: decreases clause *)
 unfold
-let sum_with_mut_borrows_decreases (max : u32) (mi : u32) (ms : u32) : nat =
+let sum_with_mut_borrows_loop_decreases (max : u32) (mi : u32) (ms : u32) : nat =
   if max >= mi then max - mi else 0
 
 (** [loops::sum_with_shared_borrows]: decreases clause *)
 unfold
-let sum_with_shared_borrows_decreases (max : u32) (i : u32) (s : u32) : nat =
+let sum_with_shared_borrows_loop_decreases (max : u32) (i : u32) (s : u32) : nat =
   if max >= i then max - i else 0
 
 (** [loops::clear]: decreases clause *)
-unfold let clear_decreases (v : vec u32) (i : usize) : nat =
+unfold let clear_loop_decreases (v : vec u32) (i : usize) : nat =
   if i <= List.Tot.length v then List.Tot.length v - i else 0
 
 (** [loops::list_mem]: decreases clause *)
-unfold let list_mem_decreases (i : u32) (ls : list_t u32) : list_t u32 =
+unfold let list_mem_loop_decreases (i : u32) (ls : list_t u32) : list_t u32 =
   ls
 
 (** [loops::list_nth_mut_loop]: decreases clause *)
 unfold
-let list_nth_mut_loop_decreases (t : Type0) (ls : list_t t) (i : u32) : nat =
+let list_nth_mut_loop_loop_decreases (t : Type0) (ls : list_t t) (i : u32) : nat =
   i
 
 (** [loops::list_nth_shared_loop]: decreases clause *)
 unfold
-let list_nth_shared_loop_decreases (t : Type0) (ls : list_t t) (i : u32) : list_t t =
+let list_nth_shared_loop_loop_decreases (t : Type0) (ls : list_t t) (i : u32) : list_t t =
   ls
 
 (** [loops::get_elem_mut]: decreases clause *)
 unfold
-let get_elem_mut_decreases (x : usize) (ls : list_t usize) : list_t usize = ls
+let get_elem_mut_loop_decreases (x : usize) (ls : list_t usize) : list_t usize = ls
 
 (** [loops::get_elem_shared]: decreases clause *)
 unfold
-let get_elem_shared_decreases (slots : vec (list_t usize)) (x : usize)
+let get_elem_shared_loop_decreases (slots : vec (list_t usize)) (x : usize)
   (ls : list_t usize) (ls0 : list_t usize) : list_t usize =
   ls
 
 (** [loops::list_nth_mut_loop_with_id]: decreases clause *)
 unfold
-let list_nth_mut_loop_with_id_decreases (t : Type0) (i : u32) (ls : list_t t) :
+let list_nth_mut_loop_with_id_loop_decreases (t : Type0) (i : u32) (ls : list_t t) :
   list_t t =
   ls
 
 (** [loops::list_nth_shared_loop_with_id]: decreases clause *)
 unfold
-let list_nth_shared_loop_with_id_decreases (t : Type0) (l : list_t t)
+let list_nth_shared_loop_with_id_loop_decreases (t : Type0) (l : list_t t)
   (i : u32) (ls : list_t t) : list_t t =
   ls
 
 (** [loops::list_nth_mut_loop_pair]: decreases clause *)
 unfold
-let list_nth_mut_loop_pair_decreases (t : Type0) (l : list_t t) (l0 : list_t t)
+let list_nth_mut_loop_pair_loop_decreases (t : Type0) (l : list_t t) (l0 : list_t t)
   (i : u32) : nat =
   i
 
 (** [loops::list_nth_shared_loop_pair]: decreases clause *)
 unfold
-let list_nth_shared_loop_pair_decreases (t : Type0) (l : list_t t)
+let list_nth_shared_loop_pair_loop_decreases (t : Type0) (l : list_t t)
   (l0 : list_t t) (i : u32) : list_t t =
   l
 
 (** [loops::list_nth_mut_loop_pair_merge]: decreases clause *)
 unfold
-let list_nth_mut_loop_pair_merge_decreases (t : Type0) (l : list_t t)
+let list_nth_mut_loop_pair_merge_loop_decreases (t : Type0) (l : list_t t)
   (l0 : list_t t) (i : u32) : nat =
   i
 
 (** [loops::list_nth_shared_loop_pair_merge]: decreases clause *)
 unfold
-let list_nth_shared_loop_pair_merge_decreases (t : Type0) (l : list_t t)
+let list_nth_shared_loop_pair_merge_loop_decreases (t : Type0) (l : list_t t)
   (l0 : list_t t) (i : u32) : list_t t =
   l
 
 (** [loops::list_nth_mut_shared_loop_pair]: decreases clause *)
 unfold
-let list_nth_mut_shared_loop_pair_decreases (t : Type0) (l : list_t t)
+let list_nth_mut_shared_loop_pair_loop_decreases (t : Type0) (l : list_t t)
   (l0 : list_t t) (i : u32) : list_t t =
   l
 
 (** [loops::list_nth_mut_shared_loop_pair_merge]: decreases clause *)
 unfold
-let list_nth_mut_shared_loop_pair_merge_decreases (t : Type0) (l : list_t t)
+let list_nth_mut_shared_loop_pair_merge_loop_decreases (t : Type0) (l : list_t t)
   (l0 : list_t t) (i : u32) : list_t t =
   l
 
 (** [loops::list_nth_shared_mut_loop_pair]: decreases clause *)
 unfold
-let list_nth_shared_mut_loop_pair_decreases (t : Type0) (l : list_t t)
+let list_nth_shared_mut_loop_pair_loop_decreases (t : Type0) (l : list_t t)
   (l0 : list_t t) (i : u32) : list_t t =
   l
 
 (** [loops::list_nth_shared_mut_loop_pair_merge]: decreases clause *)
 unfold
-let list_nth_shared_mut_loop_pair_merge_decreases (t : Type0) (l : list_t t)
+let list_nth_shared_mut_loop_pair_merge_loop_decreases (t : Type0) (l : list_t t)
   (l0 : list_t t) (i : u32) : list_t t =
   l
